CoqOfNoir/simulation/CoqOfNoir.v
@@ -1,4 +1,5 @@
 Require Import CoqOfNoir.CoqOfNoir.
+Require Import Coq.Logic.FunctionalExtensionality.
 
 Module ToValue.
   Class Trait (Self : Set) : Set := {
@@ -19,6 +20,14 @@ Module Panic.
   Definition to_result {A : Set} `{ToValue.Trait A} (value : t A) : Result.t :=
     match value with
     | Success value => Result.Ok (to_value value)
+    | Error => Result.Panic
+    end.
+
+  (** For some intermediate results, we need to make an allocation to be like in the translated
+      code *)
+  Definition to_result_alloc {A : Set} `{ToValue.Trait A} (value : t A) : Result.t :=
+    match value with
+    | Success value => Result.Ok (M.alloc (to_value value))
     | Error => Result.Panic
     end.
 
@@ -80,6 +89,15 @@ Module StatePanic.
     | [] => return_ init
     | x :: l => bind (f init x) (fun init => fold_left init l f)
     end.
+
+  Definition lift_from_panic {State A : Set} (value : Panic.t A) : t State A :=
+    fun state => (value, state).
+
+  Definition read {State : Set} : t State State :=
+    fun state => (Panic.return_ state, state).
+
+  Definition write {State : Set} (state : State) : t State unit :=
+    fun _ => (Panic.return_ tt, state).
 End StatePanic.
 
 Module StatePanicNotations.
@@ -97,6 +115,12 @@ Module StatePanicNotations.
     (at level 200, X at level 100, Y at level 200).
 
   Notation "foldS!" := StatePanic.fold_left.
+
+  Notation "return!toS!" := StatePanic.lift_from_panic.
+
+  Notation "readS!" := StatePanic.read.
+
+  Notation "writeS!" := StatePanic.write.
 End StatePanicNotations.
 
 Export PanicNotations.
@@ -107,10 +131,20 @@ Global Instance Impl_ToValue_for_unit : ToValue.Trait unit := {
     Value.Tuple [];
 }.
 
+Lemma rewrite_to_value_unit :
+  Value.Tuple [] = to_value tt.
+Proof. reflexivity. Qed.
+Global Hint Rewrite rewrite_to_value_unit : to_value.
+
 Global Instance Impl_ToValue_for_bool : ToValue.Trait bool := {
   to_value (b : bool) :=
     Value.Bool b;
 }.
+
+Lemma rewrite_to_value_bool (b : bool) :
+  Value.Bool b = to_value b.
+Proof. reflexivity. Qed.
+Global Hint Rewrite rewrite_to_value_bool : to_value.
 
 Module Field.
   Record t : Set := {
@@ -121,6 +155,11 @@ Module Field.
     to_value (i : t) :=
       Value.Integer IntegerKind.Field i.(value);
   }.
+
+  Lemma rewrite_to_value (i : t) :
+    Value.Integer IntegerKind.Field i.(value) = to_value i.
+  Proof. reflexivity. Qed.
+  Global Hint Rewrite rewrite_to_value : to_value.
 End Field.
 
 Module U1.
@@ -132,6 +171,11 @@ Module U1.
     to_value (i : t) :=
       Value.Integer IntegerKind.U1 i.(value);
   }.
+
+  Lemma rewrite_to_value (i : t) :
+    Value.Integer IntegerKind.U1 i.(value) = to_value i.
+  Proof. reflexivity. Qed.
+  Global Hint Rewrite rewrite_to_value : to_value.
 End U1.
 
 Module U8.
@@ -143,6 +187,11 @@ Module U8.
     to_value (i : t) :=
       Value.Integer IntegerKind.U8 i.(value);
   }.
+
+  Lemma rewrite_to_value (i : t) :
+    Value.Integer IntegerKind.U8 i.(value) = to_value i.
+  Proof. reflexivity. Qed.
+  Global Hint Rewrite rewrite_to_value : to_value.
 End U8.
 
 Module U16.
@@ -154,6 +203,11 @@ Module U16.
     to_value (i : t) :=
       Value.Integer IntegerKind.U16 i.(value);
   }.
+
+  Lemma rewrite_to_value (i : t) :
+    Value.Integer IntegerKind.U16 i.(value) = to_value i.
+  Proof. reflexivity. Qed.
+  Global Hint Rewrite rewrite_to_value : to_value.
 End U16.
 
 Module U32.
@@ -165,6 +219,11 @@ Module U32.
     to_value (i : t) :=
       Value.Integer IntegerKind.U32 i.(value);
   }.
+
+  Lemma rewrite_to_value (i : t) :
+    Value.Integer IntegerKind.U32 i.(value) = to_value i.
+  Proof. reflexivity. Qed.
+  Global Hint Rewrite rewrite_to_value : to_value.
 End U32.
 
 Module U64.
@@ -176,6 +235,11 @@ Module U64.
     to_value (i : t) :=
       Value.Integer IntegerKind.U64 i.(value);
   }.
+
+  Lemma rewrite_to_value (i : t) :
+    Value.Integer IntegerKind.U64 i.(value) = to_value i.
+  Proof. reflexivity. Qed.
+  Global Hint Rewrite rewrite_to_value : to_value.
 End U64.
 
 Module I1.
@@ -187,6 +251,11 @@ Module I1.
     to_value (i : t) :=
       Value.Integer IntegerKind.I1 i.(value);
   }.
+
+  Lemma rewrite_to_value (i : t) :
+    Value.Integer IntegerKind.I1 i.(value) = to_value i.
+  Proof. reflexivity. Qed.
+  Global Hint Rewrite rewrite_to_value : to_value.
 End I1.
 
 Module I8.
@@ -198,6 +267,11 @@ Module I8.
     to_value (i : t) :=
       Value.Integer IntegerKind.I8 i.(value);
   }.
+
+  Lemma rewrite_to_value (i : t) :
+    Value.Integer IntegerKind.I8 i.(value) = to_value i.
+  Proof. reflexivity. Qed.
+  Global Hint Rewrite rewrite_to_value : to_value.
 End I8.
 
 Module I16.
@@ -209,6 +283,11 @@ Module I16.
     to_value (i : t) :=
       Value.Integer IntegerKind.I16 i.(value);
   }.
+
+  Lemma rewrite_to_value (i : t) :
+    Value.Integer IntegerKind.I16 i.(value) = to_value i.
+  Proof. reflexivity. Qed.
+  Global Hint Rewrite rewrite_to_value : to_value.
 End I16.
 
 Module I32.
@@ -220,6 +299,11 @@ Module I32.
     to_value (i : t) :=
       Value.Integer IntegerKind.I32 i.(value);
   }.
+
+  Lemma rewrite_to_value (i : t) :
+    Value.Integer IntegerKind.I32 i.(value) = to_value i.
+  Proof. reflexivity. Qed.
+  Global Hint Rewrite rewrite_to_value : to_value.
 End I32.
 
 Module I64.
@@ -231,147 +315,146 @@ Module I64.
     to_value (i : t) :=
       Value.Integer IntegerKind.I64 i.(value);
   }.
+
+  Lemma rewrite_to_value (i : t) :
+    Value.Integer IntegerKind.I64 i.(value) = to_value i.
+  Proof. reflexivity. Qed.
+  Global Hint Rewrite rewrite_to_value : to_value.
 End I64.
 
-Module SemiInteger.
+Module Integer.
   Class Trait (Self : Set) : Set := {
     to_Z : Self -> Z;
-  }.
-End SemiInteger.
-
-Global Instance Impl_SemiInteger_for_Field : SemiInteger.Trait Field.t := {
-  SemiInteger.to_Z (i : Field.t) :=
-    i.(Field.value);
-}.
-
-Global Instance Impl_SemiInteger_for_U1 : SemiInteger.Trait U1.t := {
-  SemiInteger.to_Z (i : U1.t) :=
-    i.(U1.value);
-}.
-
-Global Instance Impl_SemiInteger_for_U8 : SemiInteger.Trait U8.t := {
-  SemiInteger.to_Z (i : U8.t) :=
-    i.(U8.value);
-}.
-
-Global Instance Impl_SemiInteger_for_U16 : SemiInteger.Trait U16.t := {
-  SemiInteger.to_Z (i : U16.t) :=
-    i.(U16.value);
-}.
-
-Global Instance Impl_SemiInteger_for_U32 : SemiInteger.Trait U32.t := {
-  SemiInteger.to_Z (i : U32.t) :=
-    i.(U32.value);
-}.
-
-Global Instance Impl_SemiInteger_for_U64 : SemiInteger.Trait U64.t := {
-  SemiInteger.to_Z (i : U64.t) :=
-    i.(U64.value);
-}.
-
-Global Instance Impl_SemiInteger_for_I1 : SemiInteger.Trait I1.t := {
-  SemiInteger.to_Z (i : I1.t) :=
-    i.(I1.value);
-}.
-
-Global Instance Impl_SemiInteger_for_I8 : SemiInteger.Trait I8.t := {
-  SemiInteger.to_Z (i : I8.t) :=
-    i.(I8.value);
-}.
-
-Global Instance Impl_SemiInteger_for_I16 : SemiInteger.Trait I16.t := {
-  SemiInteger.to_Z (i : I16.t) :=
-    i.(I16.value);
-}.
-
-Global Instance Impl_SemiInteger_for_I32 : SemiInteger.Trait I32.t := {
-  SemiInteger.to_Z (i : I32.t) :=
-    i.(I32.value);
-}.
-
-Global Instance Impl_SemiInteger_for_I64 : SemiInteger.Trait I64.t := {
-  SemiInteger.to_Z (i : I64.t) :=
-    i.(I64.value);
-}.
-
-Module Integer.
-  Class Trait (Self : Set) `{SemiInteger.Trait Self} : Set := {
     of_Z : Z -> Self;
+    min : Z;
+    max : Z;
   }.
-
-  Definition to_Z {Self : Set} `{Trait Self} (self : Self) : Z :=
-    SemiInteger.to_Z self.
-
-  Definition to_nat {Self : Set} `{Trait Self} (self : Self) : nat :=
-    Z.to_nat (to_Z self).
 
   Definition add {Self : Set} `{Trait Self} (self other : Self) : Self :=
-    of_Z (SemiInteger.to_Z self + SemiInteger.to_Z other).
+    of_Z (Integer.to_Z self + Integer.to_Z other).
 
   Definition sub {Self : Set} `{Trait Self} (self other : Self) : Self :=
-    of_Z (SemiInteger.to_Z self - SemiInteger.to_Z other).
+    of_Z (Integer.to_Z self - Integer.to_Z other).
 
   Definition mul {Self : Set} `{Trait Self} (self other : Self) : Self :=
-    of_Z (SemiInteger.to_Z self * SemiInteger.to_Z other).
+    of_Z (Integer.to_Z self * Integer.to_Z other).
 
   Definition div {Self : Set} `{Trait Self} (self other : Self) : Self :=
-    of_Z (SemiInteger.to_Z self / SemiInteger.to_Z other).
+    of_Z (Integer.to_Z self / Integer.to_Z other).
 
   Definition mod_ {Self : Set} `{Trait Self} (self other : Self) : Self :=
-    of_Z (SemiInteger.to_Z self mod SemiInteger.to_Z other).
+    of_Z (Integer.to_Z self mod Integer.to_Z other).
 
   Definition of_bool {Self : Set} `{Trait Self} (b : bool) : Self :=
     of_Z (if b then 1 else 0).
 End Integer.
 
 Global Instance Impl_Integer_for_U1 : Integer.Trait U1.t := {
+  Integer.to_Z (i : U1.t) :=
+    i.(U1.value);
   Integer.of_Z (i : Z) :=
     U1.Build_t (i mod (2^1));
+  Integer.min := 0;
+  Integer.max := 1;
 }.
 
 Global Instance Impl_Integer_for_U8 : Integer.Trait U8.t := {
+  Integer.to_Z (i : U8.t) :=
+    i.(U8.value);
   Integer.of_Z (i : Z) :=
     U8.Build_t (i mod (2^8));
+  Integer.min := 0;
+  Integer.max := 2^8 - 1;
 }.
 
 Global Instance Impl_Integer_for_U16 : Integer.Trait U16.t := {
+  Integer.to_Z (i : U16.t) :=
+    i.(U16.value);
   Integer.of_Z (i : Z) :=
     U16.Build_t (i mod (2^16));
+  Integer.min := 0;
+  Integer.max := 2^16 - 1;
 }.
 
 Global Instance Impl_Integer_for_U32 : Integer.Trait U32.t := {
+  Integer.to_Z (i : U32.t) :=
+    i.(U32.value);
   Integer.of_Z (i : Z) :=
     U32.Build_t (i mod (2^32));
+  Integer.min := 0;
+  Integer.max := 2^32 - 1;
 }.
 
 Global Instance Impl_Integer_for_U64 : Integer.Trait U64.t := {
+  Integer.to_Z (i : U64.t) :=
+    i.(U64.value);
   Integer.of_Z (i : Z) :=
     U64.Build_t (i mod (2^64));
+  Integer.min := 0;
+  Integer.max := 2^64 - 1;
 }.
 
 Global Instance Impl_Integer_for_I1 : Integer.Trait I1.t := {
+  Integer.to_Z (i : I1.t) :=
+    i.(I1.value);
   Integer.of_Z (i : Z) :=
     I1.Build_t (((i + 2^0) mod (2^1)) - 2^0);
+  Integer.min := -1;
+  Integer.max := 0;
 }.
 
 Global Instance Impl_Integer_for_I8 : Integer.Trait I8.t := {
+  Integer.to_Z (i : I8.t) :=
+    i.(I8.value);
   Integer.of_Z (i : Z) :=
     I8.Build_t (((i + 2^7) mod (2^8)) - 2^7);
+  Integer.min := -2^7;
+  Integer.max := 2^7 - 1;
 }.
 
 Global Instance Impl_Integer_for_I16 : Integer.Trait I16.t := {
+  Integer.to_Z (i : I16.t) :=
+    i.(I16.value);
   Integer.of_Z (i : Z) :=
     I16.Build_t (((i + 2^15) mod (2^16)) - 2^15);
+  Integer.min := -2^15;
+  Integer.max := 2^15 - 1;
 }.
 
 Global Instance Impl_Integer_for_I32 : Integer.Trait I32.t := {
+  Integer.to_Z (i : I32.t) :=
+    i.(I32.value);
   Integer.of_Z (i : Z) :=
     I32.Build_t (((i + 2^31) mod (2^32)) - 2^31);
+  Integer.min := -2^31;
+  Integer.max := 2^31 - 1;
 }.
 
 Global Instance Impl_Integer_for_I64 : Integer.Trait I64.t := {
+  Integer.to_Z (i : I64.t) :=
+    i.(I64.value);
   Integer.of_Z (i : Z) :=
     I64.Build_t (((i + 2^63) mod (2^64)) - 2^63);
+  Integer.min := -2^63;
+  Integer.max := 2^63 - 1;
+}.
+
+(** With this trait, we can take into account both standard integers and fields, whose size depends
+    on a parameter [p]. *)
+Module ToZ.
+  Class Trait (Self : Set) : Set := {
+    to_Z : Self -> Z;
+  }.
+End ToZ.
+
+Global Instance Impl_ToZ_for_Field : ToZ.Trait Field.t := {
+  ToZ.to_Z (i : Field.t) :=
+    i.(Field.value);
+}.
+
+Global Instance Impl_ToZ_for_Integer {A : Set} `{Integer.Trait A} : ToZ.Trait A := {
+  ToZ.to_Z (i : A) :=
+    Integer.to_Z i;
 }.
 
 Module Array.
@@ -383,34 +466,37 @@ Module Array.
   Arguments t : clear implicits.
   Arguments Build_t {_ _}.
 
-  Module Valid.
-    Definition t {A : Set} {size : U32.t} (array : t A size) : Prop :=
-      List.length array.(value) = Z.to_nat (SemiInteger.to_Z size).
-  End Valid.
-
   Global Instance Impl_ToValue {A : Set} `{ToValue.Trait A} {size : U32.t} :
       ToValue.Trait (t A size) := {
     to_value (array : t A size) :=
       Value.Array (List.map to_value array.(value));
   }.
 
+  Lemma rewrite_to_value {A : Set} `{ToValue.Trait A} {size : U32.t} (array : t A size) f :
+    (forall (x : A), f x = to_value x) ->
+    Value.Array (List.map f array.(value)) = to_value array.
+  Proof.
+    hauto lq: on use: functional_extensionality.
+  Qed.
+  Global Hint Rewrite @rewrite_to_value : to_value.
+
   Definition repeat {A : Set} (size : U32.t) (value : A) : t A size :=
     {|
-      value := List.repeat value (Z.to_nat (SemiInteger.to_Z size))
+      value := List.repeat value (Z.to_nat (Integer.to_Z size))
     |}.
 
-  Definition read {A Index: Set} `{SemiInteger.Trait Index} {size : U32.t}
+  Definition read {A Index: Set} `{ToZ.Trait Index} {size : U32.t}
       (array : t A size) (index : Index) :
       M! A :=
-    match List.nth_error array.(value) (Z.to_nat (SemiInteger.to_Z index)) with
+    match List.nth_error array.(value) (Z.to_nat (ToZ.to_Z index)) with
     | Some result => return! result
     | None => panic! ("Array.get: index out of bounds", array, index)
     end.
 
-  Definition write {A Index: Set} `{SemiInteger.Trait Index} {size : U32.t}
+  Definition write {A Index: Set} `{ToZ.Trait Index} {size : U32.t}
       (array : t A size) (index : Index) (update : A) :
       M! (t A size) :=
-    match List.listUpdate_error array.(value) (Z.to_nat (SemiInteger.to_Z index)) update with
+    match List.listUpdate_error array.(value) (Z.to_nat (ToZ.to_Z index)) update with
     | Some array => return! (Build_t array)
     | None => panic! ("Array.write: index out of bounds", array, index)
     end.
@@ -422,9 +508,9 @@ Module Eq.
   }.
 End Eq.
 
-Global Instance Impl_Eq_for_U8 : Eq.Trait U8.t := {
-  Eq.eq (self other : U8.t) :=
-    self.(U8.value) =? other.(U8.value);
+Global Instance Impl_Eq_for_Integer {A : Set} `{Integer.Trait A} : Eq.Trait A := {
+  Eq.eq (self other : A) :=
+    Integer.to_Z self =? Integer.to_Z other;
 }.
 
 Global Instance Impl_Eq_for_Array {A : Set} `{Eq.Trait A} {size : U32.t} :
@@ -432,3 +518,17 @@ Global Instance Impl_Eq_for_Array {A : Set} `{Eq.Trait A} {size : U32.t} :
   Eq.eq (self other : Array.t A size) :=
     List.fold_left andb (List.zip Eq.eq self.(Array.value) other.(Array.value)) true;
 }.
+
+Definition cast_to_integer {A B : Set} `{ToZ.Trait A} `{Integer.Trait B} (value : A) : M! B :=
+  let value := ToZ.to_Z value in
+  if (Integer.min <=? value) && (value <=? Integer.max) then
+    return! (Integer.of_Z value)
+  else
+    panic! ("cast: out of bounds", value).
+
+Definition cast_to_field {A : Set} `{ToZ.Trait A} (p : Z) (value : A) : M! Field.t :=
+  let value := ToZ.to_Z value in
+  if (0 <=? value) && (value <? p) then
+    return! (Field.Build_t value)
+  else
+    panic! ("cast: out of bounds", value).
